Add default type in typing environment.

src/TypEnv.v
@@ -11,31 +11,39 @@ Module TypEnv.
   (* A typing environment is a map from a variable to its type *)
   Definition t : Type := VM.t typ.
 
-  (* Return the size of a variable in a typing environment.
-     If the variable is not in the typing environment, return 0 by default. *)
-  Definition vsize (v : var) (e : t) : nat :=
+  (* The default type of a variable not in the typing environment *)
+  Definition deftyp : typ := Tuint 64.
+
+  (* Find the type of a variable in a typing environment *)
+  Definition find (v : var) (e : t) : typ :=
     match VM.find v e with
-    | None => 0
-    | Some t => sizeof_typ t
+    | None => deftyp
+    | Some ty => ty
     end.
 
-  Definition find (v : var) (e : t) : option typ := VM.find v e.
+  (* Return the size of a variable in a typing environment *)
+  Definition vsize (v : var) (e : t) : nat := sizeof_typ (find v e).
 
   Definition mem (v : var) (e : t) : bool := VM.mem v e.
 
   Definition add (v : var) (ty : typ) (e : t) := VM.add v ty e.
 
-  Lemma find_add_eq {x y ty e} : x == y -> find x (add y ty e) = Some ty.
-  Proof. exact: VM.Lemmas.find_add_eq. Qed.
+  Lemma find_add_eq {x y ty e} : x == y -> find x (add y ty e) = ty.
+  Proof. rewrite /find /add => H. by rewrite (VM.Lemmas.find_add_eq H). Qed.
 
   Lemma find_add_neq {x y ty e} : x != y -> find x (add y ty e) = find x e.
-  Proof. move/negP=> Hxy. exact: (VM.Lemmas.find_add_neq Hxy). Qed.
+  Proof.
+    move/negP=> Hxy. rewrite /find /add. by rewrite (VM.Lemmas.find_add_neq Hxy).
+  Qed.
 
-  Lemma mem_find_some v e : mem v e -> exists ty, find v e = Some ty.
-  Proof. exact: VM.Lemmas.mem_find_some. Qed.
+  Lemma vsize_add_eq {x y ty e} : x == y -> vsize x (add y ty e) = sizeof_typ ty.
+  Proof. rewrite /vsize=> H. by rewrite (find_add_eq H). Qed.
 
-  Lemma not_mem_find_none v e : ~~ mem v e -> find v e = None.
-  Proof. exact: VM.Lemmas.not_mem_find_none. Qed.
+  Lemma vsize_add_neq {x y ty e} : x != y -> vsize x (add y ty e) = vsize x e.
+  Proof. rewrite /vsize => H. by rewrite (find_add_neq H). Qed.
+
+  Lemma not_mem_find_deftyp v e : ~~ mem v e -> find v e = deftyp.
+  Proof. rewrite /find => H. by rewrite VM.Lemmas.not_mem_find_none. Qed.
 
   Lemma mem_add_eq {x y ty e} : x == y -> mem x (add y ty e).
   Proof. exact: VM.Lemmas.mem_add_eq. Qed.
@@ -43,7 +51,7 @@ Module TypEnv.
   Lemma mem_add_neq {x y ty e} : x != y -> mem x (add y ty e) = mem x e.
   Proof. move/idP/negP=> H. exact: (VM.Lemmas.mem_add_neq H). Qed.
 
-  Lemma find_some_vsize x e ty : find x e = Some ty -> vsize x e = sizeof_typ ty.
+  Lemma find_vsize x e ty : find x e = ty -> vsize x e = sizeof_typ ty.
   Proof. rewrite /vsize /find. move=> ->. reflexivity. Qed.
 
 End TypEnv.
